WIP

cava/Cava/Util/BitArithmetic.v
@@ -190,7 +190,7 @@ Module BigEndianBytes.
   (* convert a big-endian list of bytes to a list of n-byte words (length of list
    must be a multiple of n) *)
   Definition bytes_to_Ns n (x : list byte) : list N :=
-    List.map (fun i => concat_bytes (firstn n (skipn (n*i) x))) (seq 0 (length x / 4)).
+    List.map (fun i => concat_bytes (firstn n (skipn (n*i) x))) (seq 0 (length x / n)).
 End BigEndianBytes.
 
 Definition byte_xor (x y : byte) : byte := N_to_byte (N.lxor (Byte.to_N x) (Byte.to_N y)).
